Verify deleteTx

kubernetes_model/apimodel/transaction.go
@@ -1,0 +1,54 @@
+package apimodel
+
+import (
+	"fmt"
+
+	apierrors "k8s.io/apimachinery/pkg/api/errors"
+	"k8s.io/apimachinery/pkg/api/meta"
+	metav1 "k8s.io/apimachinery/pkg/apis/meta/v1"
+)
+
+func preconditionUIDMismatch(options metav1.DeleteOptions, metadata metav1.Object) bool {
+	return options.Preconditions != nil && options.Preconditions.UID != nil && *options.Preconditions.UID != metadata.GetUID()
+}
+
+func setPreconditionResourceVersion(options *metav1.DeleteOptions, metadata metav1.Object) {
+	rv := metadata.GetResourceVersion()
+	if options.Preconditions == nil {
+		options.Preconditions = &metav1.Preconditions{}
+	}
+	options.Preconditions.ResourceVersion = &rv
+}
+
+func (s *State) deleteTx(key KKey, options metav1.DeleteOptions) error {
+	for {
+		optionsCopy := *options.DeepCopy()
+
+		obj, err := s.get(key)
+		if err != nil {
+			return err
+		}
+
+		metadata, err := meta.Accessor(obj)
+		if err != nil {
+			return fmt.Errorf("failed to access object metadata: %w", err)
+		}
+
+		if preconditionUIDMismatch(optionsCopy, metadata) {
+			return newPreconditionUIDConflictError(
+				key.Kind,
+				metadata.GetName(),
+				string(*optionsCopy.Preconditions.UID),
+				string(metadata.GetUID()),
+			)
+		}
+
+		setPreconditionResourceVersion(&optionsCopy, metadata)
+
+		err = s.delete(key, optionsCopy)
+		if apierrors.IsConflict(err) {
+			continue
+		}
+		return err
+	}
+}
