src/proof/k8s_io/apimachinery/pkg/api/errors.v
@@ -1,5 +1,6 @@
 From New.proof.k8s_io.apimachinery.pkg.api Require Export errors_init.
 From New.proof Require Import prelude empty_ffi.
+From New.proof.kubernetes_model Require Import errors.
 
 Section proof.
 Context `{hG: !heapGS Σ} {go_ctx: GoContext}.
@@ -10,6 +11,28 @@ Lemma wp_IsNotFound_nil err:
   }}}
     @! errors.IsNotFound #err
   {{{ RET (#false);
+    True%I
+  }}}.
+Proof.
+Admitted.
+
+Lemma wp_IsConflict_nil err:
+  {{{ is_pkg_init code.k8s_io.apimachinery.pkg.api.errors.errors ∗
+      ⌜ err = interface.nil ⌝
+  }}}
+    @! errors.IsConflict #err
+  {{{ RET (#false);
+    True%I
+  }}}.
+Proof.
+Admitted.
+
+Lemma wp_IsConflict_conflict err:
+  {{{ is_pkg_init code.k8s_io.apimachinery.pkg.api.errors.errors ∗
+      ⌜ conflict_error err ⌝
+  }}}
+    @! errors.IsConflict #err
+  {{{ RET (#true);
     True%I
   }}}.
 Proof.
