src/proof/kubernetes_model/errors.v
@@ -1,0 +1,5 @@
+From New.proof Require Import prelude empty_ffi.
+
+Axiom conflict_error: interface.t → Prop.
+Axiom conflict_error_dec: ∀ err, Decision (conflict_error err).
+Global Existing Instance conflict_error_dec.
