src/proof/kubernetes_model/tx/delete.v
@@ -1,0 +1,583 @@
+From New.proof Require Import prelude empty_ffi.
+From New.proof.kubernetes_model Require Export delete.
+From New.proof.kubernetes_model Require Import get.
+From New.proof.k8s_io.apimachinery.pkg.api Require Import errors.
+From iris.bi.lib Require Import atomic.
+
+Section proof.
+Context `{hG: !heapGS Σ} {go_ctx: GoContext}.
+Context `{!kubernetesModelG Σ}.
+
+Definition precondition_uid_mismatch (options : DeleteOptionsV.t) (metadata : ObjectMetaV.t) : bool :=
+  match options.(DeleteOptionsV.Preconditions') with
+  | Some preconditions =>
+      match preconditions.(PreconditionsV.UID') with
+      | Some uid => bool_decide (uid ≠ metadata.(ObjectMetaV.UID'))
+      | None => false
+      end
+  | None => false
+  end.
+
+Lemma wp_preconditionUIDMismatch options_c options metadata_i metadata_l metadata dq :
+  {{{ is_pkg_init apimodel ∗
+      "%Hmetadata_i" ∷ ⌜ metadata_i = interface.mk (ptrT.id v1.ObjectMeta.id) #metadata_l ⌝ ∗
+      "Hdeepown_options" ∷ DeleteOptionsV.deepown options_c options dq ∗
+      "Hdeepown_metadata" ∷ ObjectMetaV.deepown_l metadata_l metadata dq
+  }}}
+    @! apimodel.preconditionUIDMismatch #options_c #metadata_i
+  {{{ mismatch, RET #mismatch;
+      "%Hmismatch" ∷ ⌜ mismatch = precondition_uid_mismatch options metadata ⌝ ∗
+      "Hdeepown_options" ∷ DeleteOptionsV.deepown options_c options dq ∗
+      "Hdeepown_metadata" ∷ ObjectMetaV.deepown_l metadata_l metadata dq
+  }}}.
+Proof.
+  wp_start as "H".
+  iNamed "H". subst metadata_i.
+  iNamed "Hdeepown_options".
+  destruct options.(DeleteOptionsV.Preconditions') as [preconditions|] eqn:Hpreconditions.
+  - iDestruct "Hdeepown_preconditions_some" as (preconditions_c)
+      "[Hpreconditions_l Hdeepown_preconditions]".
+    iNamed "Hdeepown_preconditions".
+    assert (v1.DeleteOptions.Preconditions' options_c ≠ null) as Hpreconditions_not_null.
+    { intros Hnull. apply (proj1 Hdeepown_preconditions_none) in Hnull. congruence. }
+    assert (bool_decide (v1.DeleteOptions.Preconditions' options_c = null) = false)
+      as Hpreconditions_nonnull_decide.
+    { apply bool_decide_false. done. }
+    wp_auto.
+    rewrite Hpreconditions_nonnull_decide /=.
+    wp_auto.
+    destruct preconditions.(PreconditionsV.UID') as [uid|] eqn:Huid.
+    + iDestruct "Hdeepown_uid_some" as (uid_c) "[Huid_l ->]".
+      assert (v1.Preconditions.UID' preconditions_c ≠ null) as Huid_not_null.
+      { intros Hnull. apply (proj1 Hdeepown_uid_none) in Hnull. congruence. }
+      assert (bool_decide (v1.Preconditions.UID' preconditions_c = null) = false)
+        as Huid_nonnull_decide.
+      { apply bool_decide_false. done. }
+      rewrite Huid_nonnull_decide /=.
+      wp_auto.
+      wp_apply (v1.wp_GetUID_deepown with "[$Hdeepown_metadata]").
+      iIntros "Hdeepown_metadata".
+      destruct (decide (uid = metadata.(ObjectMetaV.UID'))) as [Huid_eq|Huid_neq].
+      * rewrite Huid_eq.
+        wp_auto.
+        iAssert ((match preconditions.(PreconditionsV.UID') with
+          | Some vu => ∃ cu, v1.Preconditions.UID' preconditions_c ↦{dq} cu ∗ ⌜ cu = vu ⌝
+          | None => True
+          end)%I) with "[Huid_l]" as "Hdeepown_uid_some".
+        { rewrite Huid /=. iExists metadata.(ObjectMetaV.UID'). iFrame. done. }
+        iAssert (PreconditionsV.deepown preconditions_c preconditions dq)
+          with "[Hdeepown_uid_some Hdeepown_resourceversion_some]" as "Hdeepown_preconditions".
+        { rewrite /PreconditionsV.deepown Huid /=. iFrame. iPureIntro. done. }
+        iAssert ((match options.(DeleteOptionsV.Preconditions') with
+          | Some vp =>
+              ∃ cp, v1.DeleteOptions.Preconditions' options_c ↦{dq} cp ∗
+                PreconditionsV.deepown cp vp dq
+          | None => True
+          end)%I) with "[Hpreconditions_l Hdeepown_preconditions]"
+          as "Hdeepown_preconditions_some".
+        { rewrite Hpreconditions /=. iExists preconditions_c. iFrame. }
+        iAssert (DeleteOptionsV.deepown options_c options dq)
+          with "[Hdeepown_graceperiodseconds_some Hdeepown_preconditions_some Hdeepown_orphandependents_some Hdeepown_propagationpolicy_some]"
+          as "Hdeepown_options".
+        { rewrite /DeleteOptionsV.deepown Hpreconditions /=. iFrame. iPureIntro. done. }
+        iApply "HΦ". iFrame. iPureIntro.
+        rewrite /precondition_uid_mismatch Hpreconditions Huid /=.
+        rewrite Huid_eq.
+        replace (bool_decide (ObjectMetaV.UID' metadata = ObjectMetaV.UID' metadata)) with true
+          by (symmetry; apply bool_decide_true; done).
+        replace (bool_decide (ObjectMetaV.UID' metadata ≠ ObjectMetaV.UID' metadata)) with false
+          by (symmetry; apply bool_decide_false; intros Hneq; apply Hneq; done).
+        done.
+      * wp_auto.
+        iAssert ((match preconditions.(PreconditionsV.UID') with
+          | Some vu => ∃ cu, v1.Preconditions.UID' preconditions_c ↦{dq} cu ∗ ⌜ cu = vu ⌝
+          | None => True
+          end)%I) with "[Huid_l]" as "Hdeepown_uid_some".
+        { rewrite Huid /=. iExists uid. iFrame. done. }
+        iAssert (PreconditionsV.deepown preconditions_c preconditions dq)
+          with "[Hdeepown_uid_some Hdeepown_resourceversion_some]" as "Hdeepown_preconditions".
+        { rewrite /PreconditionsV.deepown Huid /=. iFrame. iPureIntro. done. }
+        iAssert ((match options.(DeleteOptionsV.Preconditions') with
+          | Some vp =>
+              ∃ cp, v1.DeleteOptions.Preconditions' options_c ↦{dq} cp ∗
+                PreconditionsV.deepown cp vp dq
+          | None => True
+          end)%I) with "[Hpreconditions_l Hdeepown_preconditions]"
+          as "Hdeepown_preconditions_some".
+        { rewrite Hpreconditions /=. iExists preconditions_c. iFrame. }
+        iAssert (DeleteOptionsV.deepown options_c options dq)
+          with "[Hdeepown_graceperiodseconds_some Hdeepown_preconditions_some Hdeepown_orphandependents_some Hdeepown_propagationpolicy_some]"
+          as "Hdeepown_options".
+        { rewrite /DeleteOptionsV.deepown Hpreconditions /=. iFrame. iPureIntro. done. }
+        iApply "HΦ". iFrame. iPureIntro.
+        rewrite /precondition_uid_mismatch Hpreconditions Huid /=.
+        replace (bool_decide (uid = ObjectMetaV.UID' metadata)) with false
+          by (symmetry; apply bool_decide_false; done).
+        replace (bool_decide (uid ≠ ObjectMetaV.UID' metadata)) with true
+          by (symmetry; apply bool_decide_true; done).
+        done.
+    + assert (v1.Preconditions.UID' preconditions_c = null) as Huid_null.
+      { apply (proj2 Hdeepown_uid_none). done. }
+      assert (bool_decide (v1.Preconditions.UID' preconditions_c = null) = true)
+        as Huid_null_decide.
+      { apply bool_decide_true. done. }
+      rewrite Huid_null_decide /=.
+      wp_auto.
+      iAssert (PreconditionsV.deepown preconditions_c preconditions dq)
+        with "[Hdeepown_resourceversion_some]" as "Hdeepown_preconditions".
+      { rewrite /PreconditionsV.deepown Huid /=. iFrame. iPureIntro. done. }
+      iAssert ((match options.(DeleteOptionsV.Preconditions') with
+        | Some vp =>
+            ∃ cp, v1.DeleteOptions.Preconditions' options_c ↦{dq} cp ∗
+              PreconditionsV.deepown cp vp dq
+        | None => True
+        end)%I) with "[Hpreconditions_l Hdeepown_preconditions]"
+        as "Hdeepown_preconditions_some".
+      { rewrite Hpreconditions /=. iExists preconditions_c. iFrame. }
+      iAssert (DeleteOptionsV.deepown options_c options dq)
+        with "[Hdeepown_graceperiodseconds_some Hdeepown_preconditions_some Hdeepown_orphandependents_some Hdeepown_propagationpolicy_some]"
+        as "Hdeepown_options".
+      { rewrite /DeleteOptionsV.deepown Hpreconditions /=. iFrame. iPureIntro. done. }
+      iApply "HΦ". iFrame. iPureIntro.
+      rewrite /precondition_uid_mismatch Hpreconditions Huid /=. done.
+  - assert (v1.DeleteOptions.Preconditions' options_c = null) as Hpreconditions_null.
+    { apply (proj2 Hdeepown_preconditions_none). done. }
+    assert (bool_decide (v1.DeleteOptions.Preconditions' options_c = null) = true)
+      as Hpreconditions_null_decide.
+    { apply bool_decide_true. done. }
+    wp_auto.
+    rewrite Hpreconditions_null_decide /=.
+    wp_auto.
+    iAssert (DeleteOptionsV.deepown options_c options dq)
+      with "[Hdeepown_graceperiodseconds_some Hdeepown_preconditions_some Hdeepown_orphandependents_some Hdeepown_propagationpolicy_some]"
+      as "Hdeepown_options".
+    { rewrite /DeleteOptionsV.deepown Hpreconditions /=. iFrame. iPureIntro. done. }
+    iApply "HΦ". iFrame. iPureIntro.
+    rewrite /precondition_uid_mismatch Hpreconditions /=. done.
+Qed.
+
+Definition delete_tx_preconditions_with_rv (options : DeleteOptionsV.t) (rv : go_string) :
+    PreconditionsV.t :=
+  match options.(DeleteOptionsV.Preconditions') with
+  | None => {|
+      PreconditionsV.UID' := None;
+      PreconditionsV.ResourceVersion' := Some rv;
+    |}
+  | Some preconditions =>
+      preconditions <| PreconditionsV.ResourceVersion' := Some rv |>
+  end.
+
+Definition delete_tx_options_with_rv (options : DeleteOptionsV.t) (rv : go_string) :
+    DeleteOptionsV.t :=
+  options <| DeleteOptionsV.Preconditions' :=
+    Some (delete_tx_preconditions_with_rv options rv) |>.
+
+Axiom delete_tx_options_with_rv_valid :
+  ∀ options rv,
+    DeleteOptionsV.valid options →
+    DeleteOptionsV.valid (delete_tx_options_with_rv options rv).
+
+Lemma delete_tx_options_with_rv_preconditions_match_uid options rv uid :
+  delete_preconditions_match_uid options uid →
+  delete_preconditions_match_uid (delete_tx_options_with_rv options rv) uid.
+Proof.
+  rewrite /delete_preconditions_match_uid /delete_tx_options_with_rv
+    /delete_tx_preconditions_with_rv.
+  destruct options.(DeleteOptionsV.Preconditions') as [preconditions|]; [|done].
+  destruct preconditions as [uid_o rv_o].
+  simpl.
+  destruct uid_o; done.
+Qed.
+
+Lemma delete_tx_options_with_rv_preconditions_match_uid_iff options rv uid :
+  delete_preconditions_match_uid (delete_tx_options_with_rv options rv) uid ↔
+  delete_preconditions_match_uid options uid.
+Proof.
+  rewrite /delete_preconditions_match_uid /delete_tx_options_with_rv
+    /delete_tx_preconditions_with_rv.
+  destruct options.(DeleteOptionsV.Preconditions') as [preconditions|]; [|done].
+  destruct preconditions as [uid_o rv_o].
+  simpl.
+  destruct uid_o; done.
+Qed.
+
+Lemma delete_tx_options_with_rv_preconditions_resource_version_not_none options rv :
+  ¬ delete_options_preconditions_resource_version_none (delete_tx_options_with_rv options rv).
+Proof.
+  rewrite /delete_options_preconditions_resource_version_none /delete_tx_options_with_rv
+    /delete_tx_preconditions_with_rv.
+  destruct options.(DeleteOptionsV.Preconditions') as [[uid_o rv_o]|]; simpl; congruence.
+Qed.
+
+Lemma precondition_uid_mismatch_false options metadata uid :
+  delete_preconditions_match_uid options uid →
+  uid = metadata.(ObjectMetaV.UID') →
+  precondition_uid_mismatch options metadata = false.
+Proof.
+  rewrite /delete_preconditions_match_uid /precondition_uid_mismatch.
+  destruct options.(DeleteOptionsV.Preconditions') as [preconditions|]; [|done].
+  destruct preconditions.(PreconditionsV.UID') as [precondition_uid|]; [|done].
+  intros Hmatch Huid_eq.
+  rewrite Hmatch Huid_eq.
+  apply bool_decide_eq_false_2.
+  intros Hneq. apply Hneq. done.
+Qed.
+
+Lemma wp_setPreconditionResourceVersion options_l options metadata_i metadata_l metadata :
+  {{{ is_pkg_init apimodel ∗
+      "%Hmetadata_i" ∷ ⌜ metadata_i = interface.mk (ptrT.id v1.ObjectMeta.id) #metadata_l ⌝ ∗
+      "Hdeepown_options_l" ∷ DeleteOptionsV.deepown_l options_l options 1 ∗
+      "Hdeepown_metadata" ∷ ObjectMetaV.deepown_l metadata_l metadata 1 }}}
+    @! apimodel.setPreconditionResourceVersion #options_l #metadata_i
+  {{{ RET #();
+      "Hdeepown_options_l" ∷ DeleteOptionsV.deepown_l options_l
+        (delete_tx_options_with_rv options metadata.(ObjectMetaV.ResourceVersion')) 1 ∗
+      "Hdeepown_metadata" ∷ ObjectMetaV.deepown_l metadata_l metadata 1 }}}.
+Proof.
+  wp_start as "H".
+  iNamed "H". subst metadata_i.
+  iDestruct "Hdeepown_options_l" as (options_c) "[Hoptions_l Hdeepown_options]".
+  iNamed "Hdeepown_options".
+  wp_auto.
+  wp_apply (v1.wp_GetResourceVersion_deepown with "[$Hdeepown_metadata]").
+  iIntros "Hdeepown_metadata".
+  wp_auto.
+  iAssert (⌜ rv_ptr ≠ null ⌝%I) as "%Hrv_ptr_not_null".
+  { iDestruct (typed_pointsto_not_null with "rv") as %H; [done|]. done. }
+  destruct options.(DeleteOptionsV.Preconditions') as [preconditions|] eqn:Hpreconditions.
+  - iDestruct "Hdeepown_preconditions_some" as (preconditions_c)
+      "[Hpreconditions_l Hdeepown_preconditions]".
+    iNamed "Hdeepown_preconditions".
+    assert (v1.DeleteOptions.Preconditions' options_c ≠ null) as Hpreconditions_not_null.
+    { intros Hnull.
+      apply (proj1 Hdeepown_preconditions_none) in Hnull.
+      congruence. }
+    assert (bool_decide (v1.DeleteOptions.Preconditions' options_c = null) = false)
+      as Hpreconditions_nonnull_decide.
+    { apply bool_decide_false. done. }
+    destruct preconditions.(PreconditionsV.UID') as [uid|] eqn:Huid.
+    + iDestruct "Hdeepown_uid_some" as (uid_c) "[Huid_l ->]".
+      rewrite Hpreconditions_nonnull_decide.
+      wp_auto.
+      iAssert (PreconditionsV.deepown
+        (preconditions_c <| v1.Preconditions.ResourceVersion' := rv_ptr |>)
+        (preconditions <| PreconditionsV.ResourceVersion' :=
+          Some metadata.(ObjectMetaV.ResourceVersion') |>) 1)%I
+        with "[Huid_l rv]" as "Hdeepown_preconditions".
+      { rewrite /PreconditionsV.deepown Huid /=.
+        iFrame. iPureIntro.
+        split; first done.
+        split; first done.
+        split; last done.
+        split; [intros Hnull; exfalso; apply Hrv_ptr_not_null; done|intros Hnone; congruence]. }
+      iAssert ((match (delete_tx_options_with_rv options
+          metadata.(ObjectMetaV.ResourceVersion')).(DeleteOptionsV.Preconditions') with
+        | Some preconditions_v =>
+            ∃ preconditions_c',
+              (options_c.(v1.DeleteOptions.Preconditions') ↦ preconditions_c') ∗
+              PreconditionsV.deepown preconditions_c' preconditions_v 1
+        | None => True
+        end)%I) with "[Hpreconditions_l Hdeepown_preconditions]" as
+        "Hdeepown_preconditions_some".
+      { rewrite /delete_tx_options_with_rv /delete_tx_preconditions_with_rv
+          Hpreconditions /=.
+        iExists (preconditions_c <| v1.Preconditions.ResourceVersion' := rv_ptr |>).
+        iFrame. }
+      iAssert (DeleteOptionsV.deepown_l options_l
+        (delete_tx_options_with_rv options metadata.(ObjectMetaV.ResourceVersion')) 1)%I
+        with "[Hoptions_l Hdeepown_graceperiodseconds_some Hdeepown_preconditions_some Hdeepown_orphandependents_some Hdeepown_propagationpolicy_some]"
+        as "Hdeepown_options_l".
+      { iExists options_c. iFrame "Hoptions_l".
+        rewrite /DeleteOptionsV.deepown /delete_tx_options_with_rv
+          /delete_tx_preconditions_with_rv Hpreconditions /=.
+        iFrame. iFrame "%".
+        iPureIntro.
+        split; [intros Hnull; exfalso; apply Hpreconditions_not_null; done|intros Hnone; congruence]. }
+      iApply "HΦ". iFrame.
+    + rewrite Hpreconditions_nonnull_decide.
+      wp_auto.
+      iAssert (PreconditionsV.deepown
+        (preconditions_c <| v1.Preconditions.ResourceVersion' := rv_ptr |>)
+        (preconditions <| PreconditionsV.ResourceVersion' :=
+          Some metadata.(ObjectMetaV.ResourceVersion') |>) 1)%I
+        with "[rv]" as "Hdeepown_preconditions".
+      { rewrite /PreconditionsV.deepown Huid /=.
+        iFrame. iPureIntro.
+        split; first done.
+        split; last done.
+        split; [intros Hnull; exfalso; apply Hrv_ptr_not_null; done|intros Hnone; congruence]. }
+      iAssert ((match (delete_tx_options_with_rv options
+          metadata.(ObjectMetaV.ResourceVersion')).(DeleteOptionsV.Preconditions') with
+        | Some preconditions_v =>
+            ∃ preconditions_c',
+              (options_c.(v1.DeleteOptions.Preconditions') ↦ preconditions_c') ∗
+              PreconditionsV.deepown preconditions_c' preconditions_v 1
+        | None => True
+        end)%I) with "[Hpreconditions_l Hdeepown_preconditions]" as
+        "Hdeepown_preconditions_some".
+      { rewrite /delete_tx_options_with_rv /delete_tx_preconditions_with_rv
+          Hpreconditions /=.
+        iExists (preconditions_c <| v1.Preconditions.ResourceVersion' := rv_ptr |>).
+        iFrame. }
+      iAssert (DeleteOptionsV.deepown_l options_l
+        (delete_tx_options_with_rv options metadata.(ObjectMetaV.ResourceVersion')) 1)%I
+        with "[Hoptions_l Hdeepown_graceperiodseconds_some Hdeepown_preconditions_some Hdeepown_orphandependents_some Hdeepown_propagationpolicy_some]"
+        as "Hdeepown_options_l".
+      { iExists options_c. iFrame "Hoptions_l".
+        rewrite /DeleteOptionsV.deepown /delete_tx_options_with_rv
+          /delete_tx_preconditions_with_rv Hpreconditions /=.
+        iFrame. iFrame "%".
+        iPureIntro.
+        split; [intros Hnull; exfalso; apply Hpreconditions_not_null; done|intros Hnone; congruence]. }
+      iApply "HΦ". iFrame.
+  - assert (v1.DeleteOptions.Preconditions' options_c = null) as Hpreconditions_null.
+    { apply (proj2 Hdeepown_preconditions_none).
+      done. }
+    assert (bool_decide (v1.DeleteOptions.Preconditions' options_c = null) = true)
+      as Hpreconditions_null_decide.
+    { apply bool_decide_true. done. }
+    rewrite Hpreconditions_null_decide.
+    wp_auto.
+    wp_alloc preconditions_ptr as "Hpreconditions_l".
+    wp_auto.
+    iClear "Hdeepown_preconditions_some".
+    iAssert (⌜ preconditions_ptr ≠ null ⌝%I) as "%Hpreconditions_ptr_not_null".
+    { iDestruct (typed_pointsto_not_null with "Hpreconditions_l") as %H; [done|]. done. }
+    iAssert (PreconditionsV.deepown
+      (v1.Preconditions.mk null rv_ptr)
+      (delete_tx_preconditions_with_rv options metadata.(ObjectMetaV.ResourceVersion')) 1)%I
+      with "[rv]" as "Hdeepown_preconditions".
+    { rewrite /PreconditionsV.deepown /delete_tx_preconditions_with_rv
+        Hpreconditions /=.
+      iFrame. iPureIntro.
+      split; first done.
+      split; last done.
+      split; [intros Hnull; exfalso; apply Hrv_ptr_not_null; done|intros Hnone; congruence]. }
+    iAssert ((match (delete_tx_options_with_rv options
+        metadata.(ObjectMetaV.ResourceVersion')).(DeleteOptionsV.Preconditions') with
+      | Some preconditions_v =>
+          ∃ preconditions_c',
+            ((options_c <| v1.DeleteOptions.Preconditions' := preconditions_ptr |>)
+              .(v1.DeleteOptions.Preconditions') ↦ preconditions_c') ∗
+            PreconditionsV.deepown preconditions_c' preconditions_v 1
+      | None => True
+      end)%I) with "[Hpreconditions_l Hdeepown_preconditions]" as
+      "Hdeepown_preconditions_some".
+    { rewrite /delete_tx_options_with_rv /delete_tx_preconditions_with_rv
+        Hpreconditions /=.
+      iExists (v1.Preconditions.mk null rv_ptr).
+      iFrame. }
+    iAssert (DeleteOptionsV.deepown_l options_l
+      (delete_tx_options_with_rv options metadata.(ObjectMetaV.ResourceVersion')) 1)%I
+      with "[Hoptions_l Hdeepown_graceperiodseconds_some Hdeepown_preconditions_some Hdeepown_orphandependents_some Hdeepown_propagationpolicy_some]"
+      as "Hdeepown_options_l".
+    { iExists (options_c <| v1.DeleteOptions.Preconditions' := preconditions_ptr |>).
+      iFrame "Hoptions_l".
+      rewrite /DeleteOptionsV.deepown /delete_tx_options_with_rv
+        /delete_tx_preconditions_with_rv Hpreconditions /=.
+      iFrame. iFrame "%".
+      iPureIntro.
+      split; [intros Hnull; exfalso; apply Hpreconditions_ptr_not_null; done|intros Hnone; congruence]. }
+    iApply "HΦ". iFrame.
+Qed.
+
+Lemma wp_State__deleteTx_au γ l key options_c options:
+  ∀ Φ,
+    is_pkg_init apimodel ∗
+    is_kubernetes γ l ∗
+    "Hdeepown_options" ∷ DeleteOptionsV.deepown options_c options 1 ∗
+    "%Hvalid_options" ∷ ⌜ DeleteOptionsV.valid options ⌝ ∗
+    "Hau" ∷ AU <{ ∃∃ uid kmeta parent_key parent_uid children,
+      "%Hkey_in" ∷ ⌜ key ∈ children ⌝ ∗
+      "%Hdelete_preconditions_uid" ∷ ⌜ delete_preconditions_match_uid options uid ⌝ ∗
+      "Hown_meta_frag" ∷ own_meta_frag γ key uid 1 kmeta ∗
+      "Hown_children_frag" ∷ own_children_frag γ parent_key parent_uid 1 children
+    }> @ ⊤, ∅ <{ ∀∀ kmeta',
+      delete_success_post γ key uid parent_key parent_uid children kmeta',
+      COMM ▷ Φ #interface.nil
+    }>
+    -∗ WP l @ (ptrT.id apimodel.State.id) @ "deleteTx" #key #options_c {{ Φ }}.
+Proof.
+  iIntros (Φ) "(#Hinit & #Hkinv & H)".
+  iNamed "H".
+  wp_method_call. wp_call. wp_auto.
+  set I := (∃ options_c_orig,
+    "Hoptions_ptr" ∷ options_ptr ↦ options_c_orig ∗
+    "Hdeepown_options_orig" ∷ DeleteOptionsV.deepown options_c_orig options 1 ∗
+    "Hau" ∷ AU <{ ∃∃ uid kmeta parent_key parent_uid children,
+      "%Hkey_in" ∷ ⌜ key ∈ children ⌝ ∗
+      "%Hdelete_preconditions_uid" ∷ ⌜ delete_preconditions_match_uid options uid ⌝ ∗
+      "Hown_meta_frag" ∷ own_meta_frag γ key uid 1 kmeta ∗
+      "Hown_children_frag" ∷ own_children_frag γ parent_key parent_uid 1 children
+    }> @ ⊤, ∅ <{ ∀∀ kmeta',
+      delete_success_post γ key uid parent_key parent_uid children kmeta',
+      COMM ▷ Φ #interface.nil
+    }>
+  )%I.
+  iAssert I with "[options Hdeepown_options Hau]" as "Hloop_inv".
+  { iExists options_c. iFrame. }
+  wp_for "Hloop_inv".
+  wp_apply (wp_DeleteOptions__DeepCopy with
+    "[Hoptions_ptr Hdeepown_options_orig]").
+  { iFrame. }
+  iIntros (options_copy_ptr) "[(%options_c_copy & Hoptions_copy_ptr & Hdeepown_options_copy)
+    (%options_c' & Hoptions_ptr & Hdeepown_options_orig)]".
+  wp_auto.
+  iClear "Hoptions_copy_ptr". clear options_copy_ptr.
+  wp_apply (wp_State__get_some_au γ l key).
+  iFrame "#".
+  iMod "Hau" as (uid kmeta parent_key parent_uid children) "[Hau_pre Hclose]".
+  iNamed "Hau_pre".
+  iDestruct "Hclose" as "[Habort _]".
+  iModIntro.
+  iExists uid, (DfracOwn 1), kmeta, None, None.
+  iFrame "Hown_meta_frag".
+  iSplit; first done.
+  iSplit; first done.
+  iIntros (i kobj) "Hget".
+  iDestruct "Hget" as "(%Hvalid_kobj & %Hkey_eq & %Hmeta_eq & Hdeepown_i & Hown_meta_frag & _ & _)".
+  iPoseProof (kview.own_meta_valid with "Hown_meta_frag") as "%Hmeta_valid".
+  iMod ("Habort" with "[Hown_meta_frag Hown_children_frag]") as "Hau".
+  { iFrame. iFrame "%". }
+  iModIntro. iNext. wp_auto.
+  iDestruct "Hdeepown_i" as (kobj_l) "[%Hvalid_interface Hdeepown_l]".
+  rewrite bool_decide_true //. wp_auto.
+  wp_apply wp_Accessor. 1: iPureIntro; done.
+  rewrite bool_decide_true //. wp_auto.
+  iPoseProof (KObjectV.deepown_l_split with "Hdeepown_l") as
+    "(Htypemeta & Hdeepown_metadata & Hdeepown_spec & Hdeepown_status)".
+  destruct Hmeta_valid as (_ & _ & Huid_kmeta & _).
+  assert (Huid_kobj : uid = (KObjectV.objectmeta kobj).(ObjectMetaV.UID')).
+  { rewrite Huid_kmeta.
+    symmetry. apply (ObjectMetaV.equiv_except_resource_version_uid _ _ Hmeta_eq). }
+  assert (Hprecondition_uid_mismatch_false :
+    precondition_uid_mismatch options (KObjectV.objectmeta kobj) = false).
+  { eapply precondition_uid_mismatch_false; done. }
+  wp_apply (wp_preconditionUIDMismatch with
+    "[$Hinit $Hdeepown_options_copy $Hdeepown_metadata]").
+  { done. }
+  iIntros (mismatch) "(%Hmismatch & Hdeepown_options_copy & Hdeepown_metadata)".
+  rewrite Hmismatch Hprecondition_uid_mismatch_false.
+  wp_auto.
+  wp_apply (wp_setPreconditionResourceVersion with
+    "[optionsCopy Hdeepown_options_copy Hdeepown_metadata]").
+  { iFrame "#".
+    iSplit; first done.
+    iSplitL "optionsCopy Hdeepown_options_copy".
+    { iExists options_c_copy. iFrame. }
+    iFrame. }
+  iIntros "Hpost".
+  iNamed "Hpost".
+  iDestruct "Hdeepown_options_l" as (options_c_rv) "[optionsCopy Hdeepown_options_rv]".
+  set (options_rv :=
+    delete_tx_options_with_rv options
+      (ObjectMetaV.ResourceVersion' (KObjectV.objectmeta kobj))).
+  assert (Hvalid_options_rv : DeleteOptionsV.valid options_rv).
+  { apply delete_tx_options_with_rv_valid. done. }
+  assert (Hdelete_preconditions_uid_rv :
+    delete_preconditions_match_uid options_rv uid).
+  { subst options_rv.
+    apply delete_tx_options_with_rv_preconditions_match_uid.
+    done. }
+  assert (Hdelete_preconditions_uid_equiv_rv :
+    ∀ uid',
+      delete_preconditions_match_uid options_rv uid' ↔
+      delete_preconditions_match_uid options uid').
+  { intros uid'.
+    subst options_rv.
+    apply delete_tx_options_with_rv_preconditions_match_uid_iff. }
+  wp_auto.
+  wp_apply (wp_State__delete_au γ l key options_c_rv options_rv).
+  iFrame "#".
+  iFrame "Hdeepown_options_rv".
+  iSplit; first done.
+  iMod "Hau" as (uid' kmeta' parent_key' parent_uid' children') "[Hau_pre Hclose]".
+  iNamed "Hau_pre".
+  iModIntro.
+  iExists uid', kmeta', parent_key', parent_uid', children'.
+  iFrame "Hown_meta_frag Hown_children_frag".
+  iSplit; first done.
+  iSplit.
+  { iPureIntro.
+    apply (proj2 (Hdelete_preconditions_uid_equiv_rv uid')).
+    done. }
+  destruct (decide (delete_options_preconditions_resource_version_none options_rv))
+    as [Hrv_none|Hrv_some].
+  { exfalso.
+    subst options_rv.
+    apply delete_tx_options_with_rv_preconditions_resource_version_not_none in Hrv_none.
+    done. }
+  iIntros (err' kmeta'') "Hdelete_post".
+  iDestruct "Hdelete_post" as "[Hsuccess|Hconflict]".
+  - iDestruct "Hsuccess" as "[%Herr Hpost]". subst err'.
+    iDestruct "Hclose" as "[_ Hcommit]".
+    iMod ("Hcommit" $! kmeta'' with "Hpost") as "HΦ".
+    iModIntro. iNext.
+    wp_auto.
+    wp_apply (wp_IsConflict_nil with "[]").
+    { done. }
+    wp_for_post.
+    iApply "HΦ".
+  - iDestruct "Hconflict" as "(%Herr_ne & %Hconflict & Hown_meta_frag & Hown_children_frag)".
+    iDestruct "Hclose" as "[Habort _]".
+    iMod ("Habort" with "[Hown_meta_frag Hown_children_frag]") as "Hau".
+    { iFrame. iFrame "%". }
+    iModIntro. iNext.
+    wp_auto.
+    wp_apply (wp_IsConflict_conflict with "[]").
+    { done. }
+    wp_for_post.
+    iFrame "s key".
+    iExists options_c'.
+    iFrame "Hoptions_ptr Hdeepown_options_orig Hau".
+Qed.
+
+Lemma wp_State__deleteTx γ l key options_c options uid kmeta parent_key parent_uid children :
+  {{{ is_pkg_init apimodel ∗
+      "#Hisk" ∷ is_kubernetes γ l ∗
+      "Hdeepown_options" ∷ DeleteOptionsV.deepown options_c options 1 ∗
+      "%Hvalid_options" ∷ ⌜ DeleteOptionsV.valid options ⌝ ∗
+      "%Hkey_in" ∷ ⌜ key ∈ children ⌝ ∗
+      "%Hdelete_preconditions_uid" ∷ ⌜ delete_preconditions_match_uid options uid ⌝ ∗
+      "Hown_meta_frag" ∷ own_meta_frag γ key uid 1 kmeta ∗
+      "Hown_children_frag" ∷ own_children_frag γ parent_key parent_uid 1 children
+  }}}
+    l @ (ptrT.id apimodel.State.id) @ "deleteTx" #key #options_c
+  {{{ kmeta', RET #interface.nil;
+      delete_success_post γ key uid parent_key parent_uid children kmeta'
+  }}}.
+Proof.
+  iIntros (Φ) "(#Hinit & H) HΦ".
+  iNamed "H".
+  iApply wp_State__deleteTx_au.
+  iFrame "#".
+  iFrame "%".
+  iFrame "Hdeepown_options".
+  iAssert (AU <{ ∃∃ uid0 kmeta0 parent_key0 parent_uid0 children0,
+      "%Hkey_in" ∷ ⌜ key ∈ children0 ⌝ ∗
+      "%Hdelete_preconditions_uid" ∷ ⌜ delete_preconditions_match_uid options uid0 ⌝ ∗
+      "Hown_meta_frag" ∷ own_meta_frag γ key uid0 1 kmeta0 ∗
+      "Hown_children_frag" ∷ own_children_frag γ parent_key0 parent_uid0 1 children0
+    }> @ ⊤, ∅ <{ ∀∀ kmeta',
+      delete_success_post γ key uid0 parent_key0 parent_uid0 children0 kmeta',
+      COMM ▷ Φ #interface.nil
+    }>)%I with "[Hown_meta_frag Hown_children_frag HΦ]" as "Hau".
+  { iAuIntro.
+    iAssert (("%Hkey_in" ∷ ⌜ key ∈ children ⌝ ∗
+      "%Hdelete_preconditions_uid" ∷ ⌜ delete_preconditions_match_uid options uid ⌝ ∗
+      "Hown_meta_frag" ∷ own_meta_frag γ key uid 1 kmeta ∗
+      "Hown_children_frag" ∷ own_children_frag γ parent_key parent_uid 1 children)%I)
+      with "[Hown_meta_frag Hown_children_frag]" as "Hpre".
+    { iFrame. iFrame "%". }
+    iAaccIntro with "Hpre".
+    - iIntros "Hpre".
+      iNamed "Hpre".
+      iFrame.
+      done.
+    - iIntros (kmeta') "Hpost".
+      iModIntro. iNext.
+      iApply ("HΦ" $! kmeta' with "Hpost"). }
+  iFrame "Hau".
+Qed.
+
+End proof.
